pulse/src/checker/Pulse.Reflection.Util.fst
@@ -309,10 +309,19 @@ let non_informative_witness_rt (u:R.universe) (a:R.term) : R.term =
   let t = pack_ln (Tv_App t (a, Q_Explicit)) in
   t
 
+let pulse_lib_gref = ["Pulse"; "Lib"; "GhostReference"]
+let mk_pulse_lib_gref_lid s = pulse_lib_gref@[s]
+let gref_lid = mk_pulse_lib_gref_lid "ref"
+
+let pulse_lib_higher_gref = ["Pulse"; "Lib"; "HigherGhostReference"]
+let mk_pulse_lib_higher_gref_lid s = pulse_lib_higher_gref@[s]
+let higher_gref_lid = mk_pulse_lib_higher_gref_lid "ref"
+
 let unit_non_informative_lid = mk_pulse_lib_core_lid "unit_non_informative"
 let prop_non_informative_lid = mk_pulse_lib_core_lid "prop_non_informative"
 let erased_non_informative_lid = mk_pulse_lib_core_lid "erased_non_informative"
 let squash_non_informative_lid = mk_pulse_lib_core_lid "squash_non_informative"
+let gref_non_informative_lid = mk_pulse_lib_gref_lid "gref_non_informative"
 
 let stt_vprop_equiv_fv =
   R.pack_fv (mk_pulse_lib_core_lid "vprop_equiv")
@@ -759,3 +768,7 @@ let mk_observability_lid l = ["PulseCore"; "Observability"; l]
 let observable_lid = mk_observability_lid "Observable"
 let unobservable_lid = mk_observability_lid "Unobservable"
 let neutral_lid = mk_observability_lid "Neutral"
+
+let mk_gref (u:R.universe) (t:R.term) : R.term =
+  let hd = R.pack_ln (R.Tv_UInst (R.pack_fv gref_lid) [u]) in
+  R.pack_ln (R.Tv_App hd (t, R.Q_Explicit))
